theories/Numbers/Cyclic/Int63/Int63Op.v
@@ -8,20 +8,20 @@
 (************************************************************************)
 (*            Benjamin Gregoire, Laurent Thery, INRIA, 2007             *)
 (************************************************************************)
-Require Export Int31Native.
+Require Export Int63Native.
 Require Import BigNumPrelude.
 Require Import Bvector.
 
 Set Vm Optimize.
 
 
-Local Open Scope int31_scope.
+Local Open Scope int63_scope.
 
 (** The number of digits as a int *)
 Definition digits := 63.
 
 (** The bigger int *)
-Definition max_int := Eval compute in 0 - 1.
+Definition max_int := Eval vm_compute in 0 - 1.
 Register max_int as PrimInline.
 
 (** Access to the nth digits *)
@@ -49,7 +49,7 @@ Definition bit i n :=  negb (is_zero ((i >> n) << (digits - 1))).
 (** Extra modulo operations *)
 Definition opp (i:int) := 0 - i.
 Register opp as PrimInline.
-Notation "- x" := (opp x) : int31_scope.
+Notation "- x" := (opp x) : int63_scope.
 
 Definition oppcarry i := max_int - i.
 Register oppcarry as PrimInline.
@@ -72,35 +72,35 @@ Definition addc_def x y :=
   let r := x + y in
   if r < x then C1 r else C0 r.
 (* the same but direct implementation for effeciancy *)
-Register addc      : int -> int -> carry int as int31_addc.
-Notation "n '+c' m" := (addc n m) (at level 50, no associativity) : int31_scope.
+Register addc      : int -> int -> carry int as int63_addc.
+Notation "n '+c' m" := (addc n m) (at level 50, no associativity) : int63_scope.
 
 Definition addcarryc_def x y :=
   let r := addcarry x y in
   if r <= x then C1 r else C0 r.
 (* the same but direct implementation for effeciancy *)
-Register addcarryc : int -> int -> carry int as int31_addcarryc.
+Register addcarryc : int -> int -> carry int as int63_addcarryc.
 
 Definition subc_def x y := 
   if y <= x then C0 (x - y) else C1 (x - y).
 (* the same but direct implementation for effeciancy *)
-Register subc      : int -> int -> carry int as int31_subc.
-Notation "n '-c' m" := (subc n m) (at level 50, no associativity) : int31_scope.
+Register subc      : int -> int -> carry int as int63_subc.
+Notation "n '-c' m" := (subc n m) (at level 50, no associativity) : int63_scope.
 
 Definition subcarryc_def x y :=
   if y < x then C0 (x - y - 1) else C1 (x - y - 1).
 (* the same but direct implementation for effeciancy *)
-Register subcarryc : int -> int -> carry int as int31_subcarryc.
+Register subcarryc : int -> int -> carry int as int63_subcarryc.
 
 Definition diveucl_def x y := (x/y, x\%y).
 (* the same but direct implementation for effeciancy *) 
-Register diveucl   : int -> int -> int * int as int31_diveucl.
+Register diveucl   : int -> int -> int * int as int63_diveucl.
 
-Register diveucl_21    : int -> int -> int -> int * int as int31_div21.
+Register diveucl_21    : int -> int -> int -> int * int as int63_div21.
 
 Definition addmuldiv_def p x y :=
   (x << p) lor (y >> (digits - p)).
-Register addmuldiv   : int -> int -> int -> int as int31_addmuldiv.
+Register addmuldiv   : int -> int -> int -> int as int63_addmuldiv.
 
 Definition oppc (i:int) := 0 -c i.
 Register oppc as PrimInline.
@@ -116,14 +116,14 @@ Definition compare_def x y :=
   if x < y then Lt 
   else if (x == y) then Eq else Gt.
 
-Register compare : int -> int -> comparison as int31_compare.
-Notation "n ?= m" := (compare n m) (at level 70, no associativity) : int31_scope.
+Register compare : int -> int -> comparison as int63_compare.
+Notation "n ?= m" := (compare n m) (at level 70, no associativity) : int63_scope.
 
 (** Exotic operations *)
 
 (** I should add the definition (like for compare) *)
-Register head0 : int -> int as int31_head0.
-Register tail0 : int -> int as int31_tail0.
+Register head0 : int -> int as int63_head0.
+Register tail0 : int -> int as int63_tail0.
 
 (** Iterators *)
 
