theories/Numbers/Cyclic/Int31/Int31.v
@@ -1,6 +1,0 @@
-Require Export Int31Native.
-Require Export Int31Op.
-Require Export Int31Axioms.
-Require Export Int31Properties.
-Require Export Cyclic31.
-Require Export Ring31.
